uniqueHeap/classifiedStep.v
@@ -4,6 +4,8 @@ Require Import Spec.
 Require Import Heap. 
 Require Import sets. 
 Require Import Coq.Sets.Ensembles. 
+Require Import hetList.
+Require Import Coq.Program.Equality.  
 
 Inductive SPEC : actionStack -> Prop :=
 |lockSpec : forall s, SPEC (locked s)
@@ -161,3 +163,40 @@ Proof.
     rewrite <- beq_nat_false_iff in H. rewrite H. exists ds. eassumption. }
   }
 Qed.
+
+Definition alength l :=
+  match l with
+      |locked l' => length l'
+      |unlocked l' => length l'
+  end. 
+
+Axiom uniqueThreadPool : forall T tid t t', 
+                           thread_lookup T tid t -> thread_lookup T tid t' -> t = t'. 
+
+Theorem monotonicActions : forall H tid H' T T' s1 s1' s2 s2' M M',
+                             spec_multistep H T H' T' ->
+                             tIn T (tid,s1,s2,M) -> tIn T' (tid,s1',s2',M') ->
+                             alength s1 + length s2 <= alength s1' + length s2'. 
+Proof.
+  intros. genDeps{tid; s1; s1'; s2; s2'; M; M'}. dependent induction H0. 
+  {intros. assert(thread_lookup p2 tid (tid,s1,s2,M)). econstructor. auto. 
+   auto. assert(thread_lookup p2 tid (tid,s1',s2',M')). econstructor. auto. 
+   auto. eapply uniqueThreadPool in H; eauto. inv H. omega. }
+  {intros. inversion H1; subst. 
+   {assert(tIn (tUnion T t') (tid,s1,s2,M)). constructor; auto. eapply IHspec_multistep in H4. 
+    eauto. eauto. }
+   {inversion H; subst. 
+    {inv H3. eapply IHspec_multistep. apply Union_intror. constructor. eauto. }
+    {inv H3. eapply IHspec_multistep with(s4 := aCons (fAct M E M0 d)s1)(s3:=s2) in H2. 
+     destruct s1; simpl in *; omega. apply Union_intror. apply Couple_l. }
+    {inv H3. eapply IHspec_multistep with(s4:=aCons (rAct x M E d)s1)(s3:=s2) in H2. 
+     destruct s1; simpl in *; omega. apply Union_intror. constructor. }
+    {inv H3. eapply IHspec_multistep with(s4:=aCons (wAct x M E N d)s1)(s3:=s2) in H2. 
+     destruct s1; simpl in *; omega. apply Union_intror. constructor. }
+    {inv H3. eapply IHspec_multistep with(s4:=aCons(nAct M E d x)s1)(s3:=s2) in H2. 
+     destruct s1; simpl in *; omega.  apply Union_intror. constructor. }
+    {inv H3. eapply IHspec_multistep with(s4:=aCons(srAct M E M0 N d)s1)(s3:=s2) in H2.
+     destruct s1; simpl in *; omega. apply Union_intror. constructor. }
+   }
+  }
+Qed. 
